Start first cache proof

timing/examples/data_structures/array/cache/binary/cache.c
@@ -1,0 +1,15 @@
+#include "../../../../timing_experiments.h"
+
+uint32_t sum(uint32_t* arr, uint32_t size) {
+    int x = 0;
+    for (int i = 0; i < size; i++) {
+        x += arr[i];
+    }
+    return x;
+}
+
+uint32_t cached_sum(uint32_t* arr1, uint32_t* arr2, uint32_t size) {
+    uint32_t x = sum(arr1, 1000);
+    x += sum(arr2, 1000);
+    return x;
+}
