timing/examples/data_structures/array/cache/binary/cache.h
@@ -1,0 +1,7 @@
+#ifndef CACHE
+#define CACHE
+#include "../../../../timing_experiments.h"
+
+uint32_t cached_sum(uint32_t* arr1, uint32_t* arr2, uint32_t size);
+
+#endif /* CACHE */
