timing/examples/data_structures/array/cache/binary/main.c
@@ -1,0 +1,15 @@
+#include "cache.h"
+
+int main(int argc, char* argv[]) {
+    uint32_t arr[1000];
+    
+    for (uint32_t j = 0; j < 100; j++) {
+    	for(uint32_t i = 0; i < 1000; i++) {
+	        arr[i] = rand();
+	    }
+	
+	    printf("%d\n", cached_sum(arr, arr, 1000));
+    }
+
+    return 0;
+}
