timing/examples/data_structures/array/cache/cached_sum_proofs.v
@@ -1,0 +1,126 @@
+Require Import cached_sum.
+Require Import RISCVTiming.
+Import RISCVNotations.
+
+Module TimingProof (cpu : CPUTimingBehavior).
+
+Module Program_cached_sum <: ProgramInformation.
+    Definition entry_addr : N := 0x210.
+
+    Definition exits (t:trace) : bool :=
+        match t with (Addr a,_)::_ => match a with
+        | 0x250 => true
+        | _ => false
+    end | _ => false end.
+
+    Definition binary := cached_sum.
+End Program_cached_sum.
+
+Module RISCVTiming := RISCVTiming cpu Program_cached_sum.
+Module cached_sumAuto := RISCVTimingAutomation RISCVTiming.
+Import Program_cached_sum cached_sumAuto.
+
+Definition sum (low high : N) (f : N -> N) : N :=
+    let range := List.map N.of_nat (List.seq (N.to_nat low) (N.to_nat (high - low))) in
+    List.fold_left (fun acc i => acc + f i) range 0.
+
+Lemma sum_0_0 : forall f, sum 0 0 f = 0.
+Proof. reflexivity. Qed.
+
+Lemma sum_Sn : forall low high f,
+    low <= high ->
+    sum low (1 + high) f = sum low high f + f high.
+Proof.
+    intros. unfold sum at 1.
+    rewrite <- N.add_sub_assoc, N.add_1_l, N2Nat.inj_succ.
+    rewrite seq_S, map_app, fold_left_app. simpl.
+    rewrite N2Nat.inj_sub at 2.
+    rewrite Arith_base.le_plus_minus_r_stt by lia.
+    rewrite N2Nat.id. reflexivity. assumption.
+Qed.
+
+Lemma sum_sub1 : forall low high body,
+    low < high ->
+    sum low (high - 1) (fun _ => body) + body = 
+        sum low high (fun _ => body).
+Proof.
+    intros. unfold sum at 2.
+    destruct (high - low) eqn:E using N.peano_ind.
+    - lia.
+    - clear IHn. rewrite N2Nat.inj_succ, seq_S, map_app, fold_left_app.
+      simpl. unfold sum. now replace n with (high - 1 - low) by lia.
+Qed.
+
+Definition time_of_cached_sum (ra sp size : N) (arr : addr) (c c' : cache) (t : trace) :=
+    cycle_count_of_trace t c = (
+        taddi + tsw false (sp ⊖ 12) + taddi + taddi + tsw false (sp ⊖ 4) + 
+            tsw false (sp ⊖ 8) + tjal false 0x1e4 +
+        (* first call to sum *)
+        (taddi + taddi + taddi + sum 0 size (fun i =>
+                ttbne (0 <? i) 0x1f8 + tslli 0x2 +
+                tadd + tlw false (arr ⊕ (i * 4)) + taddi + tadd +
+                tjalr (0 <? i) 0x1f0
+            )
+        ) +
+        taddi + taddi + taddi + tjal true 0x1e4 +
+        (* second call to sum *)
+        (taddi + taddi + taddi + sum 0 size (fun i =>
+                ttbne true 0x1f8 + tslli 0x2 +
+                tadd + tlw true (arr ⊕ (i * 4)) + taddi + tadd +
+                tjalr true 0x1f0
+            )
+        ) +
+        tlw true (sp ⊖ 4) + taddi + tlw true (sp ⊖ 8) + tlw true (sp ⊖ 12) +
+        taddi + tjalr false ra
+    , c').
+
+Definition cached_sum_timing_invs
+    (sp : N) (arr : addr) (c : cache) (t:trace) : option Prop :=
+let size := 1000 in
+match t with (Addr a, s) :: t' => match a with
+| 0x210 => Some (s R_A0 = arr /\ s R_A1 = arr /\ s R_SP = sp /\
+                    cycle_count_of_trace t' c = (0, c))
+| 0x228 => Some (exists c1 c2,
+                    s R_A0 = arr /\ s R_A1 = 1000 /\
+                    s V_MEM32 Ⓓ[sp ⊖ 4] = s R_RA /\
+                    cycle_count_of_trace t' c1 = 
+                        (taddi + tsw false (sp ⊖ 12) + taddi + taddi + 
+                        tsw false (sp ⊖ 4) + tsw false (sp ⊖ 8), c2))
+| 0x250 => Some (exists c', time_of_cached_sum (s R_RA) sp size arr c c' t)
+| _ => None end | _ => None end.
+
+Theorem cached_sum_timing:
+  forall s (t : trace) s' x' sp arr
+         (* boilerplate *)
+         (ENTRY: startof t (x',s') = (Addr entry_addr, s))
+         (MDL: models rvtypctx s)
+         (* bindings *)
+         (SP: s R_SP = sp)
+         (A0: s R_A0 = arr)
+         (A1: s R_A1 = arr),
+  satisfies_all 
+    lifted_prog
+    (cached_sum_timing_invs sp arr clear_cache)
+    exits
+  ((x',s')::t).
+Proof using.
+    intros.
+    apply prove_invs.
+    Local Ltac step := tstep r5_step.
+
+    simpl. rewrite ENTRY. unfold entry_addr. step. 
+    now repeat split.
+
+    intros.
+    eapply startof_prefix in ENTRY; try eassumption.
+    eapply preservation_exec_prog in MDL; 
+        try eassumption; [idtac|apply lift_riscv_welltyped].
+    clear - ENTRY PRE MDL. rename t1 into t. rename s1 into s'.
+
+    destruct_inv 32 PRE.
+
+    destruct PRE as (A0 & A1 & SP & Cycles).
+    - do 6 step. step.
+Qed.
+
+End TimingProof.
