timing/examples/data_structures/array/cache/binary/build.sh
@@ -1,0 +1,1 @@
+make clean_all exe RISCV_PREFIX=riscv32-unknown-elf-
